src/QueueInterface.v
@@ -1,5 +1,5 @@
 (* Instantiate Interfaces with BankersQueue *)
-From Coq Require Import List.
+From Coq Require Import List Lia.
 From Clairvoyance Require Import Core Approx ApproxM List Misc BankersQueue Cost Interfaces.
 
 Import ListNotations.
@@ -13,11 +13,13 @@ Set Maximal Implicit Insertion.
   fun q => MkQueueA (nfrontA q) Undefined (nbackA q) Undefined.
 
 #[global] Instance BottomIsLeast_QueueA {a} : BottomIsLeast (QueueA a).
-Admitted.
+Proof.
+  intros []; constructor; constructor.
+Qed.
 
 Definition a := nat.
 Definition value := Queue a.
-Definition valueA := QueueA a.
+Definition valueA := T (QueueA a).
 Notation stack := (list value) (only parsing).
 Notation stackA := (list valueA) (only parsing).
 
@@ -52,18 +54,31 @@ Definition budget : Budget :=
 
 Definition exec : Exec :=
   fun (o : op) (args : list valueA) => match o, args with
-  | Empty, _ => let! q := emptyA in ret [q]
-  | Push x, q :: _ => let! q' := pushA (Thunk q) (Thunk x) in ret [q']
+  | Empty, _ => let! q := emptyA in ret [Thunk q]
+  | Push x, q :: _ => let! q' := pushA q (Thunk x) in ret [Thunk q']
   | Pop, q :: _ =>
-    let! pop_q := popA (Thunk q) in
+    let! pop_q := popA q in
     match pop_q with
     | None => ret []
-    | Some (x, q) => let! q := force q in ret [q]
+    | Some (x, q) => ret [q]
     end
   | _, _ => ret []
   end.
 
 #[export] Existing Instances eval budget exec.
+
+#[export] Instance wf : WellFormed value := BankersQueue.well_formed.
+
+#[export] Instance wf_eval : WfEval.
+Proof.
+  red. intros [] vs Hvs; cbn.
+  - constructor; [ apply well_formed_empty | constructor ].
+  - destruct Hvs; constructor; [ | constructor ].
+    apply well_formed_push. auto.
+  - destruct Hvs; [ constructor | ].
+    destruct pop as [ [] | ] eqn:Epop; [ | constructor ].
+    constructor; [ | constructor]. eapply well_formed_pop; eauto.
+Qed.
 
 Lemma monotonic_exec (o : op) : Monotonic (exec o).
 Proof.
@@ -72,12 +87,11 @@ Proof.
   - destruct E as [ | ? ? ? ? E1 E].
     + reflexivity.
     + apply bind_mon; [ apply pushA_mon; reflexivity + auto | intros; apply ret_mon ].
-      constructor; [ auto | constructor ].
+      repeat constructor; auto.
   - destruct E as [ | ? ? ? ? E1 E ]; [ reflexivity | ].
     apply bind_mon; [ apply popA_mon; auto | intros ? ? []; [ reflexivity | ] ].
     destruct x1, y0.
-    apply bind_mon; [ apply force_mon, H | intros ].
-    apply ret_mon. constructor; [ assumption | constructor ].
+    apply ret_mon. repeat constructor; apply H.
 Qed.
 
 Definition approx_algebra : ApproxAlgebra.
@@ -88,22 +102,128 @@ Lemma well_defined_exec : WellDefinedExec.
 Proof. constructor; exact monotonic_exec. Qed.
 #[export] Existing Instance well_defined_exec.
 
+Definition onThunk {a b} (y : b) (f : a -> b) (u : T a) : b :=
+  match u with
+  | Undefined => y
+  | Thunk x => f x
+  end.
+
 (* "debt" in BankersQueue *)
 Definition potential : Potential := (* ... *)
-  fun qA => 2 * sizeX 0 (frontA qA) - 2 * nbackA qA.
+  onThunk 0 (fun qA => 2 * sizeX 0 (frontA qA) - 2 * nbackA qA).
 #[export] Existing Instance potential.
+
+Lemma subadditive_onThunk {a} `{LessDefined a, Lub a} (f : a -> nat) `{!SubadditiveMeasure f}
+  : SubadditiveMeasure (onThunk 0 f).
+Proof.
+  red. intros ? ? [? [ H1 H2 ] ]; inv H1; inv H2; cbn; [lia .. | ].
+  apply subadditive_measure. eauto.
+Qed.
 
 Lemma well_defined_potential : WellDefinedPotential.
 Proof.
-  constructor; [ apply @LubDebt_QueueA | exact (fun _ => eq_refl) ].
+  constructor.
+  - apply @subadditive_onThunk. apply @LubDebt_QueueA.
+  - exact (fun _ => eq_refl).
 Qed.
 #[export] Existing Instance well_defined_potential.
 
+Lemma less_defined_onThunk {a b} `{Exact b a, LessDefined a, BottomOf a, !BottomIsLeast a} (x : T a) (y : b)
+  : x `less_defined` exact y -> onThunk (bottom_of (exact y)) (fun x => x) x `less_defined` exact y.
+Proof.
+  intros Hy; inv Hy; cbn; [ apply bottom_is_least | auto ].
+Qed.
+
+Lemma less_defined_onThunk_inv {a} `{LessDefined a, BottomOf a, !BottomIsLeast a}
+    (x : T a) (y y' : a)
+  : onThunk y' (fun x => x) x `less_defined` y -> x `less_defined` Thunk y.
+Proof.
+  intros Hy; destruct x; constructor. apply Hy.
+Qed.
+
+Lemma pushD_val (q : Queue a) x outD :
+  let qA := fst (Tick.val (pushD q x outD)) in
+  (qA, Thunk x) = Tick.val (pushD q x outD).
+Proof.
+  destruct (Tick.val (pushD q x outD)) eqn:Ev; cbn; f_equal.
+  unfold pushD in Ev. cbn in Ev. destruct (Tick.val (mkQueueD _ _ _ _ _)) in Ev.
+  cbn in Ev. inv Ev. auto.
+Qed.
+
 Theorem physicist's_argument : Physicist'sArgument.
 Proof.
-  red.
-Admitted.
+  red. intros [] vs Hvs output Houtput; cbn [exec].
+  - exists (bottom_of (exact vs)).
+    split; [ apply bottom_is_least | ].
+    unfold emptyA; mgo_.
+    split; [ assumption | ].
+    replace (sumof _ _) with 0.
+    2: symmetry; apply (potential_bottom_list (approx_algebra := approx_algebra) potential_bottom _).
+    lia.
+  - destruct vs; cbn [eval] in Houtput.
+    { exists []; split; [ constructor | ].
+      mgo_. split; auto. lia. }
+    inv Houtput. inv H3.
+    exists (fst (Tick.val (pushD v x (onThunk (bottom_of (exact (push v x))) (fun q => q) x0))) :: bottom_of (exact vs)).
+    split.
+    { constructor.
+      { apply pushD_approx. inv H2; cbn. { apply bottom_is_least. } { assumption. } }
+      { apply bottom_is_least. } }
+    mgo_.
+    inv Hvs.
+    relax.
+    { eapply pushA_cost'.
+      - eassumption.
+      - apply less_defined_onThunk in H2. exact H2.
+      - apply pushD_val.
+      - reflexivity. }
+    cbn beta; intros ? ? [HH1 HH2]. change (debt (a := T _)) with potential in HH2.
+    replace (debt (onThunk _ _ _)) with (potential x0) in HH2.
+    2:{ destruct x0; reflexivity. }
+    mgo_.
+    split.
+    { constructor; [ | constructor ]. revert HH1. apply less_defined_onThunk_inv. }
+    remember (potential _).
+    replace (sumof _ _) with 0; [ lia | ].
+    symmetry; apply (sumof_bottom (Hf_bottom := @potential_bottom _ _ _ _ well_defined_potential)).
+  - destruct vs; cbn [eval] in Houtput.
+    { exists []; split; [ constructor | ].
+      mgo_. split; auto. lia. }
+    pose (outD := match output with [] => None | q :: _ => Some (@Undefined a, q) end).
+    pose (inD := Tick.val (popD v outD)).
+    exists (inD :: bottom_of (exact vs)).
+    split.
+    { constructor.
+      + apply popD_approx.
+        destruct pop as [ [] | ]; inv Houtput.
+        { constructor; constructor; constructor + assumption. }
+        { constructor. }
+      + apply bottom_is_least. }
+    mgo_.
+    inv Hvs.
+    relax.
+    { eapply (popA_cost' (outD := outD)).
+      - eassumption.
+      - destruct pop as [ [] | ]; inv Houtput.
+        + constructor. constructor; [ constructor | ]. auto.
+        + constructor.
+      - reflexivity. }
+    cbn beta.
+    intros ? ? [HH1 HH2].
+    change (debt (Tick.val (popD v outD))) with (potential inD) in HH2.
+    destruct pop as [ [] | ]; inv Houtput.
+    + inv HH1. inv H5. destruct y. mgo_.
+      split; [ constructor; [apply H0 | constructor ] | ].
+      change (debt x0) with (potential x0) in HH2.
+      replace (sumof _ _) with 0; [ lia | ].
+      symmetry; apply (sumof_bottom (Hf_bottom := @potential_bottom _ _ _ _ well_defined_potential)).
+    + inv HH1. mgo_. split; [ constructor | ].
+      replace (sumof _ _) with 0; [ lia | ].
+      symmetry; apply (sumof_bottom (Hf_bottom := @potential_bottom _ _ _ _ well_defined_potential)).
+Qed.
 #[export] Existing Instance physicist's_argument.
 
 Theorem amortized_cost : AmortizedCostSpec.
 Proof. apply physicist's_method. Qed.
+
+(* Print Assumptions amortized_cost. *)
